Some cleanup in Gthunks.

theories/Gthunks.v
@@ -1,112 +1,138 @@
 From stdpp Require Import namespaces.
 From iris.base_logic.lib Require Import na_invariants.
-From iris.algebra Require Import auth excl agree csum.
+From iris.algebra Require Import auth excl excl_auth agree csum.
 From iris_time Require Import TimeCredits Auth_max_nat Thunks.
 From iris_time Require Import ThunksCode.
 
-Definition genid := nat.
+(* -------------------------------------------------------------------------- *)
 
-Definition gen_ns (id : genid) : namespace :=
-  nroot .@ "gthunk" .@ id.
+(* A short theory of generations. *)
 
-(* auxiliary definition *)
-Fixpoint gens_upto' (id : genid) : coPset :=
-  match id with
+(* A generation is a natural integer. *)
+
+Definition generation := nat.
+
+Implicit Type g : generation.
+
+(* To each generation, corresponds a namespace. *)
+
+Local Definition gen_ns g : namespace :=
+  nroot .@ "gthunk" .@ g.
+
+(* The union of the namespaces of all generations in [0, g). *)
+
+Local Fixpoint gens_below_gen g : coPset :=
+  match g with
   | O => ∅
-  | S id' => gens_upto' id' ∪ ↑(gen_ns id')
+  | S g' => gens_below_gen g' ∪ ↑(gen_ns g')
   end.
 
-(* A set of generations.
-   If the bound is [Some id], this corresponds to the set [0, id);
-   If the bound is [None], then this corresponds to [0, +oo). *)
-Definition gens_upto (bound : option genid) : coPset :=
+(* A bound is an optional generation.
+   The bound [Some g] encodes the interval [0, g).
+   The bound [None] encodes the infinite set [0, +∞). *)
+
+Implicit Type bound : option generation.
+
+(* The union of the namespaces of all generations in [0, bound). *)
+
+Local Definition gens_below_bound bound : coPset :=
   match bound with
   | None => ⊤
-  | Some id => gens_upto' id
+  | Some g => gens_below_gen g
   end.
 
-(* Compare an identifier with a bound. In other words, this checks whether the
-   generation [id] is in the set [gens_upto bound]. *)
-Definition is_upto (id : genid) (bound : option genid) : Prop :=
+(* [lies_below g bound] determines whether [g] is less than [bound]. *)
+
+Local Definition lies_below g bound : Prop :=
   match bound with
   | None => True
-  | Some id' => id < id'
+  | Some g' => g < g'
   end.
 
-Lemma gen_ns_disj_upto' (n n' : genid) :
-  n ≤ n' →
-  ↑gen_ns n' ## gens_upto' n.
+(* If [g ≤ g'] holds, then the namespace associated with [g'] is disjoint
+   with the union of namespaces [gens_below_gen g]. *)
+
+Local Lemma gen_ns_disj_gens_below_gen g g' :
+  g ≤ g' →
+  ↑gen_ns g' ## gens_below_gen g.
 Proof.
-  revert n'; induction n; cbn; intros n'.
+  revert g'; induction g; cbn; intros g'.
   - set_solver.
-  - intros Hn'. rewrite disjoint_union_r. split.
-    + eapply IHn. lia.
-    + unfold gen_ns. assert (n ≠ n') by lia. solve_ndisj.
+  - intros Hg'. rewrite disjoint_union_r. split.
+    + eapply IHg. lia.
+    + unfold gen_ns. assert (g ≠ g') by lia. solve_ndisj.
 Qed.
 
-Lemma gens_upto'_mono (id id' : genid) :
-  id ≤ id' →
-  gens_upto' id ⊆ gens_upto' id'.
+(* [gens_below_gen] is monotonic. *)
+
+Local Lemma gens_below_gen_mono g g' :
+  g ≤ g' →
+  gens_below_gen g ⊆ gens_below_gen g'.
 Proof.
-  revert id; induction id'; intros id Hid; cbn.
-  - assert (id = 0) by lia; by subst id.
-  - destruct (decide (id = S id')).
-    + subst id. cbn. done.
-    + specialize (IHid' id ltac:(lia)). set_solver.
+  revert g; induction g'; intros g Hg; cbn.
+  - assert (g = 0) by lia; by subst g.
+  - destruct (decide (g = S g')).
+    + subst g. cbn. done.
+    + specialize (IHg' g ltac:(lia)). set_solver.
 Qed.
 
-Lemma gen_ns_sub_upto (id id' : genid) :
-  id < id' →
-  ↑gen_ns id ⊆ gens_upto' id'.
+(* If [g < g'] holds, then the namespace associated with [g] is contained
+   in the union of namespaces [gens_below_gen g']. *)
+
+Local Lemma gen_ns_subseteq_gens_below_gen g g' :
+  g < g' →
+  ↑gen_ns g ⊆ gens_below_gen g'.
 Proof.
-  intros Hid.
-  assert (HH: ↑gen_ns id ⊆ gens_upto' (S id)).
+  intros Hg.
+  assert (HH: ↑gen_ns g ⊆ gens_below_gen (S g)).
   { cbn. set_solver. }
-  transitivity (gens_upto' (S id)); auto.
-  by apply gens_upto'_mono.
+  transitivity (gens_below_gen (S g)); auto.
+  by apply gens_below_gen_mono.
 Qed.
+
+(* -------------------------------------------------------------------------- *)
 
 Section Gthunks.
 
   Notation valO := (valO heap_lang).
   Context `{timeCreditHeapG Σ}.
-  Context `{inG Σ (csumR (exclR unitO) (agreeR valO))}. (* γ *)
-  Context `{inG Σ (authR $ optionUR $ exclR boolO)}.    (* γforced *)
+  Context `{inG Σ (excl_authR boolO)}.                  (* γforced *)
   Context `{inG Σ (authR max_natUR)}.                   (* γpaid *)
+  Context `{inG Σ (csumR (exclR unitO) (agreeR valO))}. (* γdecided *)
   Context `{na_invG Σ}.
+  Notation iProp := (iProp Σ).
 
   Implicit Type p : na_inv_pool_name.
-  Implicit Type id : genid.
-  Implicit Type γ : gname.
   Implicit Type t : loc.
   Implicit Type n m k : nat.
   Implicit Type f : val.
 
-  Definition own_gens_upto p (bound : option genid) :=
-    na_own p (gens_upto bound).
+  Definition own_gens_below_bound p bound :=
+    na_own p (gens_below_bound bound).
 
-  Lemma own_gens_upto_alloc : ⊢ |==> ∃ p, own_gens_upto p None.
+  Local Lemma own_gens_below_alloc :
+    ⊢ |==> ∃ p, own_gens_below_bound p None.
   Proof using. iApply na_alloc. Qed.
 
   (* TODO parameterize with R *)
-  Definition Gthunk p id γ t n φ : iProp Σ :=
-    Thunk p (gen_ns id) γ t n
-            (own_gens_upto p (Some id)) φ.
+  Definition Gthunk p g γ t n φ : iProp :=
+    Thunk p (gen_ns g) γ t n
+            (own_gens_below_bound p (Some g)) φ.
 
-  Instance Gthunk_persistent p id γ t n φ :
-    Persistent (Gthunk p id γ t n φ).
+  Global Instance Gthunk_persistent p g γ t n φ :
+    Persistent (Gthunk p g γ t n φ).
   Proof using. exact _. Qed.
 
-  Lemma Gthunk_weaken p id γ t n₁ n₂ φ :
+  Lemma Gthunk_weaken p g γ t n₁ n₂ φ :
     (n₁ ≤ n₂)%nat →
-    Gthunk p id γ t n₁ φ -∗
-    Gthunk p id γ t n₂ φ.
+    Gthunk p g γ t n₁ φ -∗
+    Gthunk p g γ t n₂ φ.
   Proof using. iIntros (?) "H". by iApply Thunk_weaken. Qed.
 
-  Lemma Gthunk_consequence p id γ t n m φ ψ :
+  Lemma Gthunk_consequence p g γ t n m φ ψ :
     (∀ v, TC m -∗ φ v ={⊤}=∗ □ ψ v) -∗
-    Gthunk p id γ t  n    φ  ={∅}=∗
-    Gthunk p id γ t (n+m) ψ.
+    Gthunk p g γ t  n    φ  ={∅}=∗
+    Gthunk p g γ t (n+m) ψ.
   Proof using.
     iIntros "H1 H2".
     iApply (Thunk_consequence with "[H1] H2").
@@ -116,43 +142,43 @@ Section Gthunks.
     iAssumption.
   Qed.
 
-  Lemma Gthunk_pay E p id γ t n k φ :
+  Lemma Gthunk_pay E p g γ t n k φ :
     ↑thunkPayN t ⊆ E →
-    TC k -∗ Gthunk p id γ t n φ ={E}=∗ Gthunk p id γ t (n-k) φ.
+    TC k -∗ Gthunk p g γ t n φ ={E}=∗ Gthunk p g γ t (n-k) φ.
   Proof using. iIntros (?) "H1 H2". by iMod (Thunk_pay with "H1 H2"). Qed.
 
-  Lemma create_spec p id n φ f :
+  Lemma create_spec p g n φ f :
     TC_invariant -∗
-    {{{ TC 3 ∗ ( TC n -∗ own_gens_upto p (Some id) -∗
-                 ∀ ψ, (∀ v, own_gens_upto p (Some id) -∗ □ φ v -∗ ψ «v»%V) -∗
+    {{{ TC 3 ∗ ( TC n -∗ own_gens_below_bound p (Some g) -∗
+                 ∀ ψ, (∀ v, own_gens_below_bound p (Some g) -∗ □ φ v -∗ ψ «v»%V) -∗
                  WP «f #()» {{ ψ }} ) }}}
     « create f »
-    {{{ γ t, RET #t ; Gthunk p id γ t n φ }}}.
+    {{{ γ t, RET #t ; Gthunk p g γ t n φ }}}.
   Proof using.
     iIntros "#HtickInv" (Φ) "!# H Post".
     by wp_apply (Thunks.create_spec with "HtickInv H").
   Qed.
 
-  Lemma force_spec p id bound γ t φ :
-    is_upto id bound →
+  Lemma force_spec p g bound γ t φ :
+    lies_below g bound →
     TC_invariant -∗
-    {{{ TC 11 ∗ Gthunk p id γ t 0 φ ∗ own_gens_upto p bound }}}
+    {{{ TC 11 ∗ Gthunk p g γ t 0 φ ∗ own_gens_below_bound p bound }}}
     « force #t »
-    {{{ v, RET «v» ; ThunkVal γ v ∗ □ φ v ∗ own_gens_upto p bound }}}.
+    {{{ v, RET «v» ; ThunkVal γ v ∗ □ φ v ∗ own_gens_below_bound p bound }}}.
   Proof using.
-    intros Hid. iIntros "#HtickInv" (Φ) "!# (TC & H & Hgens) HΦ".
-    rewrite /own_gens_upto.
-    assert (gens_upto bound = gens_upto' id ∪ (gens_upto bound ∖ gens_upto' id)) as Hsplit_gens.
+    intros Hg. iIntros "#HtickInv" (Φ) "!# (TC & H & Hgens) HΦ".
+    rewrite /own_gens_below_bound.
+    assert (gens_below_bound bound = gens_below_gen g ∪ (gens_below_bound bound ∖ gens_below_gen g)) as Hsplit_gens.
     { apply union_difference_L. destruct bound.
-      + apply gens_upto'_mono. cbn in Hid. lia.
+      + apply gens_below_gen_mono. cbn in Hg. lia.
       + cbn. set_solver. }
     rewrite Hsplit_gens. iDestruct (na_own_union with "Hgens") as "[Hgens Hthunk]".
     { set_solver. }
-    assert (↑gen_ns id ⊆ gens_upto bound ∖ gens_upto' id) as Hthunk.
-    { apply subseteq_difference_r. by apply gen_ns_disj_upto'. destruct bound.
-      + by apply gen_ns_sub_upto.
+    assert (↑gen_ns g ⊆ gens_below_bound bound ∖ gens_below_gen g) as Hthunk.
+    { apply subseteq_difference_r. by apply gen_ns_disj_gens_below_gen. destruct bound.
+      + by apply gen_ns_subseteq_gens_below_gen.
       + cbn. set_solver. }
-    wp_apply (Thunks.force_spec _ p (gen_ns id) with "HtickInv [$TC $H $Hthunk $Hgens]").
+    wp_apply (Thunks.force_spec _ p (gen_ns g) with "HtickInv [$TC $H $Hthunk $Hgens]").
       by auto.
     iIntros (?) "(? & ? & Hthunk & Hgens)". iApply "HΦ". iFrame.
     iDestruct (na_own_union with "[$Hgens $Hthunk]") as "?". set_solver. done.
